src/sequent.lean
@@ -4,58 +4,317 @@ import data.multiset
 open ALC
 open ALC.Concept
 
-inductive Label (AR : Type) : Type
-  | Forall : (Role AR) → Label
-  | Exists : (Role AR)  → Label
+-- the labeled concepts 
 
--- to use with lists, we need an instance for inhabited, that is
--- to say that we have at leasts one element of the type
+inductive Label : Type
+  | Forall : Role  → Label
+  | Exists : Role  → Label
 
-/--
-instance Label_inhabited {AC AR : Type} : 
-  inhabited (Label AC AR) := inhabited.mk Label.Empty
-
-instance Concept_inhabited {AC AR : Type} :
-  inhabited (Concept AC AR) := inhabited.mk Concept.Top
-
-instance LConcept_inhabited {AC AR : Type} :
-  inhabited (LConcept AC AR) := inhabited.mk (LConcept.mk [Label.Empty] Concept.Top)
---/
-
-structure LConcept (AC AR: Type) :=
-mk :: (roles : list (Label AR))
-      (concept : Concept AC AR)
+structure LConcept : Type :=
+mk :: (roles : list Label)
+      (concept : Concept)
 
 open LConcept
 open Label
 
-@[reducible]
-def sigma' {AC AR : Type} : LConcept AC AR → Concept AC AR
-  | { LConcept . roles := [] , concept := c} := c
-  | { LConcept . roles := (Forall r :: ls) , concept := c} := (Every r (sigma' (LConcept.mk ls c)))
-  | { LConcept . roles := (Exists r :: ls) , concept := c} := (Some r (sigma' (LConcept.mk ls c)))
+def isAx : Label → Prop
+ | (Forall _) := true
+ | (Exists _) := false
 
-inductive c : Type
- | man : c
- | woman : c
+def isEx : Label → Prop
+ | (Forall _) := false
+ | (Exists _) := true
 
-inductive r : Type
- | hasChild : r
+def every {a : Type} : (a → Prop) → (list a) → Prop 
+ | f []      := true
+ | f (x::xs) := (f x) ∧ (every f xs) 
 
--- TODO : o que tá rolando??
-#reduce sigma' (LConcept.mk [@Label.Forall r (Role.Atomic r.hasChild)] (@Concept.Bot c r))
+def negLabel : list Label → list Label
+  | [] := []
+  | ((Forall a)::L) := Exists a :: negLabel L
+  | ((Exists a)::L) := Forall a :: negLabel L
+ 
+
+#check (⟨[Forall R#0, Exists R#1], (Concept.Bot)⟩ : LConcept)
 
 
-#check multiset.fold (Concept.Intersection) Concept.Top {Concept.Top}
+open LConcept
+open Label
 
---#check Concept.rec
---instance Concept_Intersection_is_commutative {AC AR : Type}:
---  @is_commutative (Concept AC AR) Concept.Intersection := ⟨λ a b, by⟩
+def sigma_aux : list Label -> Concept -> Concept 
+ | []                 c := c
+ | ((Forall r) :: ls) c := Every r (sigma_aux ls c)
+ | ((Exists r) :: ls) c := Some r (sigma_aux ls c)
 
---this is the idea for the implementation, we can use folds in multiset, but I still have to prove commutative to
---use it, but I am having trouble as it is...
+def sigma' : LConcept -> Concept
+ | ⟨ roles , concept ⟩ := sigma_aux roles concept
 
-def inter_LConcepts {AC AR : Type} (as : list (LConcept AC AR)) :=
+#reduce sigma' (⟨[Forall R#0, Exists R#1], (Concept.Bot)⟩)
+
+
+-- sequent calculus for ALC 
+
+structure Sequent : Type :=
+mk :: (lhs : list LConcept)
+      (rhs : list LConcept)
+
+local infix ` ⇒ `:51 := Sequent.mk -- \=> 
+
+#check [LConcept.mk [Forall R#0] (Concept.Bot)] ⇒ [LConcept.mk [Forall R#0, Exists R#1] (Concept.Bot)]
+
+
+#check list.map (λ x, LConcept.mk (Forall R#1 :: LConcept.roles x) (x.concept)) [LConcept.mk [Forall R#0] (Concept.Bot)]
+
+
+inductive proof : list Sequent → Sequent → Type 
+  infix ` ⊢ ` : 25 := proof
+  | ax : ∀ Ω α,                 Ω ⊢ [α] ⇒ [α] 
+  | ax_theory : ∀ Ω s,  (s ∈ Ω) → Ω ⊢ s          -- the only real use of Ω
+  | ax_falsum : ∀ Ω α,          Ω ⊢  [⟨ [], ⊥ ⟩] ⇒ [α] 
+
+  | weak_l : ∀ Ω Δ Γ δ,       Ω ⊢ (Δ ⇒ Γ) → Ω ⊢ (δ::Δ) ⇒ Γ
+  | weak_r : ∀ Ω Δ Γ γ,         Ω ⊢ (Δ ⇒ Γ) → Ω ⊢ Δ ⇒ (γ::Γ)
+
+  | contraction_l : ∀ Ω Δ Γ δ,  Ω ⊢ (δ::δ::Δ) ⇒ Γ → Ω ⊢ (δ::Δ) ⇒ Γ
+  | contraction_r : ∀ Ω Δ Γ γ,  Ω ⊢ Δ ⇒ (γ::γ::Γ) → Ω ⊢ Δ ⇒ (γ::Γ)
+
+  | perm_l : ∀ Ω Δ₁ Δ₂ Γ δ₁ δ₂,  Ω ⊢ Δ₁ ++ (δ₁ :: δ₂ :: Δ₂) ⇒ Γ →  Ω ⊢ Δ₁ ++ (δ₂::δ₁::Δ₂) ⇒ Γ
+  | perm_r : ∀ Ω Δ Γ₁ Γ₂ γ₁ γ₂,  Ω ⊢ Δ ⇒ Γ₁ ++ (γ₁::γ₂::Γ₂) → Ω ⊢ Δ ⇒ Γ₁ ++ (γ₂::γ₁::Γ₂)
+
+  | cut : ∀ Ω Δ₁ Δ₂ Γ₁ Γ₂ α,     Ω ⊢ Δ₁ ⇒ α :: Γ₁ → Ω ⊢ α :: Δ₂ ⇒ Γ₂ → Ω ⊢ Δ₁ ++ Δ₂ ⇒ Γ₁ ++ Γ₂
+
+  | and_l : ∀ Ω Δ Γ α β L, (every isAx L) → 
+            Ω ⊢ (⟨L, α⟩ :: ⟨L,β⟩ :: Δ) ⇒ Γ →  
+            Ω ⊢ (⟨ L, α ⊓ β⟩ :: Δ) ⇒ Γ
+
+  | and_r : ∀ Ω₁ Ω₂ Δ Γ α β L, (every isAx L) → 
+            Ω₁ ⊢ Δ ⇒ (⟨L, α⟩ :: Γ) →  
+            Ω₂ ⊢ Δ ⇒ (⟨L, β⟩ :: Γ) →  
+            Ω₁ ++ Ω₂ ⊢ Δ ⇒ (⟨L, α ⊓ β⟩ :: Γ) 
+
+  | all_r : ∀ Ω Δ Γ L α R,  Ω ⊢ Δ ⇒ ⟨ L ++ [Forall R], α⟩ :: Γ →
+                            Ω ⊢ Δ ⇒ ⟨ L, Ax R : α⟩ :: Γ
+  
+  | all_l : ∀ Ω Δ Γ L α R,  Ω ⊢ ⟨ L ++ [Forall R], α⟩ :: Δ ⇒ Γ →
+                            Ω ⊢ ⟨ L, Ax R : α ⟩ :: Δ ⇒ Γ
+                        
+  | exists_r : ∀ Ω Δ Γ L α R,  Ω ⊢ Δ ⇒ ⟨ (Exists R) :: L, α⟩ :: Γ →
+                               Ω ⊢ Δ ⇒ ⟨ L, Ex R : α⟩ :: Γ
+
+  | or_l : ∀ Ω Δ Γ α β L, (every isEx L) → 
+            Ω ⊢ Δ ⇒ (⟨L, α⟩ :: Γ) →  
+            Ω ⊢ Δ ⇒ (⟨L, β⟩ :: Γ) →  
+            Ω ⊢ Δ ⇒ (⟨L, α ⊔ β⟩ :: Γ) 
+
+  | or_r : ∀ Ω Δ Γ α β L, (every isEx L) → 
+            Ω ⊢ Δ ⇒ ⟨L, α⟩ :: ⟨L,β⟩ :: Γ →  
+            Ω ⊢ Δ ⇒ ⟨L, α ⊓ β⟩ :: Γ
+
+  | neg_l : ∀ Ω Δ Γ α L L1, L1 = negLabel L →  Ω ⊢ Δ ⇒ ⟨L,α⟩ :: Γ → Ω ⊢ ⟨L1, ¬ₐα⟩ :: Δ ⇒ Γ
+
+  | neg_r : ∀ Ω Δ Γ α L L1, L1 = negLabel L →  Ω ⊢ Δ ++ [⟨L,α⟩]  ⇒ Γ → Ω ⊢ Δ ⇒ ⟨L1, ¬ₐα⟩ :: Γ
+  
+  | prom_ex : ∀ Ω δ Γ R, Ω ⊢ [δ] ⇒ Γ → 
+                Ω ⊢ [⟨ Exists R :: LConcept.roles δ, LConcept.concept δ⟩] ⇒ 
+                    (list.map (λ x, ⟨ (Exists R) :: LConcept.roles x, LConcept.concept x⟩) Γ)
+
+  | prom_ax : ∀ Ω γ Δ R, Ω ⊢ Δ ⇒ [γ] → 
+                Ω ⊢ (list.map (λ x, ⟨ Forall R :: LConcept.roles x, LConcept.concept x ⟩) Δ) ⇒ 
+                    [⟨ Forall R :: LConcept.roles γ, LConcept.concept γ⟩]
+infix ` ⊢ ` := proof -- \vdash
+
+
+def doctor := C#1
+def child  := R#1
+
+lemma l1 : proof [] ([LConcept.mk [Forall child] doctor] ⇒ [LConcept.mk [Forall child] doctor]) :=
+begin
+  have S := proof.ax [] ⟨[] , doctor⟩,
+  exact proof.prom_ax [] _ _ child S,
+end
+
+lemma l2 : proof [] ([⟨[], ⊤⟩, LConcept.mk [Forall child] doctor] ⇒ [LConcept.mk [Forall child] doctor]) :=
+begin
+  apply proof.weak_l,
+  exact l1,  
+end
+
+example : proof [] ([⟨[], ⊤⟩] ⇒ [LConcept.mk [Exists R#1] (Concept.Negation C#1), LConcept.mk [Forall R#1] C#1]) :=
+begin
+  have S₁ := proof.ax [] ⟨ [] , C#1 ⟩,
+  have S₂ := proof.prom_ax _ _ _ R#1 S₁, simp at S₂,
+  have J₁ := proof.weak_l ⟨[],⊤⟩ S₂,
+  exact proof.neg_r [] [LConcept.mk [] ⊤ ] _ J₁,
+end
+
+example : proof [] ([⟨[], ⊤⟩] ⇒ 
+  [LConcept.mk [] (Concept.Some R#1 (Concept.Negation C#1)), LConcept.mk [Forall R#1] C#1]) :=
+begin
+  have S₁ := proof.ax [] ⟨ [] , C#1 ⟩,
+  have S₂ := proof.prom_ax R#1 S₁, simp at S₂,
+  have J₁ := proof.weak_l ⟨[],⊤⟩ S₂,
+  have J₂ := proof.neg_r [LConcept.mk [] ⊤ ] J₁,
+  exact proof.exists_r J₂,
+end
+
+example : proof [] ([⟨[], ⊤⟩] ⇒ 
+  [LConcept.mk [] (Concept.Some R#1 (Concept.Negation C#1)), LConcept.mk [Forall R#1] C#1]) :=
+begin
+  have S₁ := proof.ax [] ⟨ [] , C#1 ⟩,
+  have S₂ := proof.prom_ax _ _ _ R#1 S₁, simp at S₂,
+  have J₁ := proof.weak_l [] [{roles := [Forall R#1], concept := C#1}] [{roles := [Forall R#1], concept := C#1}] ⟨[],⊤⟩ S₂,
+  have J₂ := proof.neg_r [] [{roles := ([] : list Label), concept := ⊤}] [{roles := [Forall R#1], concept := C#1}] C#1 [Forall R#1] [Exists R#1] _ J₁,
+  clear S₁ S₂ J₁,
+  exact proof.exists_r [] [⟨[], ⊤⟩] [{roles := [Forall R#1], concept := C#1}] [] (¬ₐ C#1) R#1 J₂,
+  tauto,
+end
+
+example : proof [] 
+   ([LConcept.mk ([] : list Label) (Ex R#1 : ⊤)] ⇒ 
+   [(LConcept.mk [Exists R#1] ¬ₐ C#1), (LConcept.mk [Exists R#1,Forall R#1] C#1)]) := 
+begin
+ apply proof.neg_r [] 
+  [{roles := ([] : list Label), concept := Ex R#1:⊤}] 
+  [{roles := [Exists R#1, Forall R#1], concept := C#1}] C#1 [Forall R#1] [Exists R#1],
+ rw [negLabel, negLabel],
+
+ sorry
+  
+end
+
+lemma in_map {α β} {x : α} {A : list α} (x ∈ A) (f : α → β) : (f x) ∈ (list.map f A) :=
+begin
+  finish,
+end
+
+lemma head_out_map {α β} {a : α } {A : list α} {f : α → β} : list.map f (a::A) = (f a) :: list.map f A :=
+begin
+  finish,
+end
+
+def foldl_head {α} : (α → α → α) → list α → α
+  | f (a::ls) := f a (foldl_head f (ls))
+
+lemma fold_trivial {α} {a : α} {ls : list α} {f : α → α → α}: foldl_head f (a::ls) = f a (foldl_head f ls) :=
+begin
+  refl,
+end
+
+def foldl_inter : list LConcept → Concept
+  | [] := ⊤
+  | ls := foldl_head (⊓) (list.map sigma' ls)
+
+def foldl_union : list LConcept → Concept
+  | [] := ⊥
+  | ls := foldl_head (⊔) (list.map sigma' ls) 
+
+def sets_relation {α} {A C : set α} {B : set α} : A ⊆ C → (A ∩ B) ⊆ C :=
+begin
+  intro h, have h1 : A ∩ B ⊆ A, exact set.inter_subset_left A B, exact set.subset.trans h1 h,
+end
+
+def sets_relation2 {α} {A C : set α} {B : set α} : A ⊆ C → A ⊆ B ∪ C :=
+begin
+  intro h, have h1 : C ⊆ B ∪ C, exact set.subset_union_right B C, exact set.subset.trans h h1,
+end
+
+def seq_to_stmt : Sequent → Statement
+  | (Δ ⇒ Γ) := Statement.Subsumption (foldl_inter Δ) (foldl_union Γ)
+
+lemma conclusion_sub {Δ Γ I} ( δ : LConcept) : (interp_stmt I (seq_to_stmt(Δ ⇒ Γ))) →  (interp_stmt I (seq_to_stmt(δ::Δ ⇒ Γ))) :=
+begin
+  intro a,
+  induction Δ with δ₁ Δ₂ Δh, 
+  
+  induction Γ with γ₁ Γ₂ Γh,
+
+  unfold seq_to_stmt interp_stmt foldl_union interp at *,
+  rw ← set.eq_empty_of_subset_empty a, exact set.subset_univ (interp I (foldl_inter [δ])),
+
+  unfold seq_to_stmt interp_stmt interp at *, 
+  rw (set.eq_univ_of_univ_subset a), exact (interp I (foldl_inter [δ])).subset_univ,
+
+  induction Γ with γ₁ Γ₂ Γh,
+
+  unfold seq_to_stmt interp_stmt interp foldl_inter at *, rw head_out_map, unfold1 foldl_head,
+  unfold interp, rw set.inter_comm, exact sets_relation a,
+  
+  unfold seq_to_stmt interp_stmt foldl_union foldl_inter at *, rw head_out_map, unfold1 foldl_head,
+  unfold1 interp, rw set.inter_comm, exact sets_relation a,
+end
+
+
+lemma conclusion_sub_right {Δ Γ I} ( γ : LConcept) : (interp_stmt I (seq_to_stmt(Δ ⇒ Γ))) →  (interp_stmt I (seq_to_stmt(Δ ⇒ γ::Γ))) :=
+begin
+  intro a,
+  induction Δ with δ₁ Δ₂ Δh, 
+  
+  induction Γ with γ₁ Γ₂ Γh,
+
+  unfold seq_to_stmt interp_stmt foldl_union interp at *,
+  rw set.eq_empty_of_subset_empty a, exact (interp I (foldl_head has_sup.sup (list.map sigma' [γ]))).empty_subset,
+
+  unfold seq_to_stmt interp_stmt interp foldl_union at *, rw head_out_map, unfold1 foldl_head interp, 
+  rw set.eq_univ_of_univ_subset a, finish,
+
+  induction Γ with γ₁ Γ₂ Γh,
+
+  unfold seq_to_stmt interp_stmt interp foldl_union at *, rw set.eq_empty_of_subset_empty a,
+  exact set.empty_subset (interp I (foldl_head has_sup.sup (list.map sigma' [γ]))),
+
+  unfold seq_to_stmt interp_stmt foldl_union foldl_inter at *, rw head_out_map, rw head_out_map,
+  nth_rewrite 1 fold_trivial, unfold interp, exact sets_relation2 a,
+end
+
+
+theorem soundness {Ω : list Sequent} : ∀ {Δ Γ}, (proof Ω (Δ ⇒ Γ)) →  models (list.map seq_to_stmt Ω) (seq_to_stmt (Δ ⇒ Γ))
+  | _ _ (proof.ax Ω₁ α₁) := 
+    by {unfold models, intros h1 h2, unfold seq_to_stmt at *, unfold interp_stmt,}
+  | _ _ (proof.ax_theory Ω₁ (lhs ⇒ rhs) S) :=
+    by {unfold models, intros h1 h2, unfold satisfies at h2,
+     have h3 := h2 (seq_to_stmt(lhs ⇒ rhs )), 
+     have h4 := in_map (lhs ⇒ rhs) S seq_to_stmt, 
+     exact h2 (seq_to_stmt(lhs ⇒ rhs )) h4, exact (lhs ⇒ rhs),
+     }
+  | _ _ (proof.ax_falsum Ω₁ α₁) :=
+    by {unfold models, intros h1 h2, unfold seq_to_stmt at *, unfold interp_stmt,}
+  | _ _ (proof.weak_l Ω₁ Δ Γ δ h) :=
+    by { unfold models, intros I h2, unfold satisfies at h2, have h3 := h2 (seq_to_stmt(Δ ⇒ Γ)),
+      have h4 := soundness h, unfold models at h4, have h5 := h4 I, unfold satisfies at h5, have h6 := h5 h2,
+      exact conclusion_sub δ h6,
+    }
+  | _ _ (proof.weak_r Ω₁ Δ Γ γ h) :=
+    by { unfold models, intros I h2, unfold satisfies at h2, have h3 := h2 (seq_to_stmt(Δ ⇒ Γ)),
+      have h4 := soundness h, unfold models at h4, have h5 := h4 I, unfold satisfies at h5, have h6 := h5 h2,
+      exact conclusion_sub_right γ h6,
+    }
+
+/-
+reserve infix ` ⊢ `:26
+
+inductive Sequent : list LConcept → list LConcept → Type
+infix ⊢ := Sequent
+  | One : ∀ L, L ⊢ L
+  | Neg : ∀ L, [LConcept.mk [] Concept.Bot] ⊢ L
+  | Ins : ∀ L₁ A, A ∈ L₁ → L₁ ⊢ [A]
+  | WeL : ∀ L₁ L₂ A, A ∈ L₁ → L₁ ⊢ L₂ → A::L₁ ⊢ L₂
+  | WeR : ∀ L₁ L₂ B, B ∈ L₂ → L₁ ⊢ L₂ → L₁ ⊢ B::L₂
+  | CoL : ∀ L₁ L₂ A, A::A::L₁ ⊢ L₂ → (A::L₁) ⊢ L₂ 
+  | CoR : ∀ L₁ L₂ B, L₁ ⊢ (B::L₂) → L₁ ⊢ (B::L₂)
+  | PeL : ∀ AL₁ A₁ B₁ BL₁ L₂, AL₁ ++ [A₁,B₁] ++ BL₁ ⊢ L₂ →  AL₁ ++ [B₁,A₁] ++ BL₁ ⊢ L₂
+  | PeR : ∀ AL₂ A₂ B₂ BL₂ L₁, L₁ ⊢ AL₂ ++ [A₂,B₂] ++ BL₂ →  L₁ ⊢ AL₂ ++ [B₂,A₂] ++ BL₂
+  | CuT : ∀ AL₁ BL₁ B AL₂ CL₂, AL₁ ⊢ BL₁ ++ [B] → B::AL₂ ⊢ CL₂ → AL₁ ++ AL₂ ⊢ BL₁ ++ CL₂  
+
+
+#check Sequent
+
+instance Concept_Intersection_is_commutative {AC AR : Type}:
+  @is_commutative (Concept AC AR) Concept.Intersection := ⟨λ a b, by⟩
+
+this is the idea for the implementation, we can use folds in multiset, but I still have to prove commutative to
+use it, but I am having trouble as it is...
+
+def inter_LConcepts {AC AR : Type} (as : list (qLConcept AC AR)) :=
   list.foldl (Concept.Intersection) (sigma_exhaust (list.head as)) (list.map sigma_exhaust (list.tail as))
 
 def union_LConcepts {AC AR : Type} (as : list (LConcept AC AR)) :=
@@ -67,18 +326,6 @@ def sequent {AC AR : Type} (as : list (LConcept AC AR)) (bs : list (LConcept AC 
 #reduce list.foldl (λ x y, Concept.Intersection x y) (Concept.Top) [Concept.Bot]
 
 
-#reduce 4 ∈ [1,2,3]
-
-#check 4 ∈ [1,2,3]
-
-lemma l1 : 2 ∈ [1,2,3] :=
-begin
- simp,
-end
-
-#check l1
-
-
 lemma weak_l_srule {AC AR : Type} {as bs : list (LConcept AC AR)} 
   (a : LConcept AC AR) (h1 : list.mem a as) (h : subsequent as bs) : subsequent (a::as) bs :=
 begin
@@ -88,10 +335,6 @@ begin
   have hn : interp I (inter_LConcepts as) ⊆ interp I (union_LConcepts bs), from h I,
   
 end 
-
-
-
-/--
 
 pure logic! Sequent Calculus:
 
@@ -106,4 +349,4 @@ h1 : Man |- Person
 h2 : Person |- Casado
 cut h1 h2 : Man |- Casado
 
---/
+-/
